theories/L6_PCPS/assumptions.v
@@ -1,0 +1,8 @@
+From CertiCoq Require Import L6.uncurry_proto L6.shrink_proto L6.inline_proto.
+
+Goal True. idtac "---------- rw_uncurry assumptions ----------". Abort.
+Print Assumptions rw_uncurry.
+Goal True. idtac "---------- rw_inline assumptions ----------". Abort.
+Print Assumptions rw_inline.
+Goal True. idtac "---------- rw_shrink assumptions ----------". Abort.
+Print Assumptions rw_shrink.
